move induction to it's own file

Alg/ListProps/Sorted/Intersect.lean
@@ -1,185 +1,7 @@
-import Alg.ListProps.Sorted
-import Alg.Nat.Add.Cmp
-
-@[simp]
-def len (list: List α) : nat := match list with
-  | [] => nat.zero
-  | _::xs => nat.inc (len xs)
-
-def List.sorted_intersect.induction.bounded
-  [Compare α] 
-  {P: List α -> List α -> Sort _}
-  (empty_left: ∀bs, P [] bs)
-  (empty_right: ∀as, P as [])
-  (induct_lt: ∀a as b bs, Compare.ord a b = Order.Less -> P as (b::bs) -> P (a::as) (b::bs))
-  (induct_eq: ∀a as b bs, Compare.ord a b = Order.Eq -> P as bs -> P (a::as) (b::bs))
-  (induct_gt: ∀a as b bs, Compare.ord a b = Order.Greater -> P (a::as) bs -> P (a::as) (b::bs))
-  (as bs: List α) (fuel: nat) (fuel_def: len as + len bs < fuel) : P as bs := by
-  match fuel with
-  | nat.zero => 
-    have := (nat.not_lt_zero _) fuel_def
-    contradiction
-  | .inc .zero =>
-    match as, bs with
-    | [], [] => exact empty_left []
-    | x::xs, _ =>
-      have fuel_def := by
-        unfold len at fuel_def
-        rw [nat.add_inc_left] at fuel_def
-        exact ((nat.not_lt_zero _) (nat.of_lt_inc_irr fuel_def))
-      exact fuel_def.elim 
-    | _, x::xs =>
-      have fuel_def := by
-        unfold len at fuel_def
-        rw [nat.add_inc_right] at fuel_def
-        exact ((nat.not_lt_zero _) (nat.of_lt_inc_irr fuel_def))
-      exact fuel_def.elim
-  | .inc (.inc fuel) =>
-  match as with
-  | [] => exact empty_left bs
-  | a::as' => match bs with
-    | [] => exact empty_right (a::as')
-    | b::bs' => match h:Compare.ord a b with
-      | .Less => 
-      have := List.sorted_intersect.induction.bounded
-        empty_left empty_right induct_lt induct_eq induct_gt
-          as' (b::bs') fuel.inc (by
-          conv at fuel_def => {
-            lhs
-            lhs
-            unfold len
-          }
-          rw [nat.add_inc_left] at fuel_def
-          exact fuel_def)
-      apply induct_lt
-      repeat assumption
-      | .Eq => 
-        have := (List.sorted_intersect.induction.bounded 
-          empty_left empty_right induct_lt induct_eq induct_gt
-          as' bs' fuel (by
-          unfold len at fuel_def
-          rw [nat.add_inc_right, nat.add_inc_left] at fuel_def
-          exact fuel_def))
-        apply induct_eq
-        repeat assumption
-      | .Greater =>
-        have := List.sorted_intersect.induction.bounded
-          empty_left empty_right induct_lt induct_eq induct_gt
-          (a::as') bs' fuel.inc (by
-          conv at fuel_def => {
-            lhs
-            rhs
-            unfold len
-          }
-          rw [nat.add_inc_right] at fuel_def
-          exact fuel_def)
-        apply induct_gt
-        repeat assumption
-
-#print axioms List.sorted_intersect.induction.bounded
-
-theorem List.sorted_intersect.induction.bounded.fuel_irr
-  [Compare α] 
-  {P: List α -> List α -> Sort _}
-  (empty_left: ∀bs, P [] bs)
-  (empty_right: ∀as, P as [])
-  (induct_lt: ∀a as b bs, Compare.ord a b = Order.Less -> P as (b::bs) -> P (a::as) (b::bs))
-  (induct_eq: ∀a as b bs, Compare.ord a b = Order.Eq -> P as bs -> P (a::as) (b::bs))
-  (induct_gt: ∀a as b bs, Compare.ord a b = Order.Greater -> P (a::as) bs -> P (a::as) (b::bs))
-  (as bs: List α) (x y: nat) (x_def: len as + len bs < x) (y_def: len as + len bs < y) :
-  List.sorted_intersect.induction.bounded 
-    empty_left empty_right induct_lt induct_eq induct_gt as bs x x_def =
-  List.sorted_intersect.induction.bounded 
-    empty_left empty_right induct_lt induct_eq induct_gt as bs y y_def := by
-  unfold bounded
-  match x with
-  | .zero =>
-    have := bounded.proof_1 as bs
-    contradiction
-  | .inc .zero =>
-    simp
-    match y with
-    | .zero => 
-      have := bounded.proof_1 as bs
-      contradiction
-    | .inc .zero => rfl
-    | .inc (.inc y) =>
-      simp
-      match as, bs with
-      | [], [] =>
-        rfl
-      | a::as, bs =>
-        have := bounded.proof_2 a as bs
-        contradiction
-      | as, b::bs =>
-        have := bounded.proof_3 as b bs
-        contradiction
-  | .inc (.inc x) =>
-  match y with
-  | .zero =>
-    have := bounded.proof_1 as bs
-    contradiction
-  | .inc .zero =>
-    simp
-    match as, bs with
-    | [], [] =>
-      rfl
-    | a::as, bs =>
-      have := bounded.proof_2 a as bs
-      contradiction
-    | as, b::bs =>
-      have := bounded.proof_3 as b bs
-      contradiction
-  | .inc (.inc y) =>
-  match as, bs with
-  | [], _ => rfl
-  | a::as, [] => rfl
-  | a::as, b::bs =>
-  simp
-  split
-  rw [bounded.fuel_irr _ _ _ _ _ _ _ x.inc y.inc]
-  rw [bounded.fuel_irr _ _ _ _ _ _ _ x y]
-  rw [bounded.fuel_irr _ _ _ _ _ _ _ x.inc y.inc]
-
-#print axioms List.sorted_intersect.induction.bounded.fuel_irr
-
-def List.sorted_intersect.induction
-  [Compare α] 
-  {P: List α -> List α -> Sort _}
-  (empty_left: ∀bs, P [] bs)
-  (empty_right: ∀as, P as [])
-  (induct_lt: ∀a as b bs, Compare.ord a b = Order.Less -> P as (b::bs) -> P (a::as) (b::bs))
-  (induct_eq: ∀a as b bs, Compare.ord a b = Order.Eq -> P as bs -> P (a::as) (b::bs))
-  (induct_gt: ∀a as b bs, Compare.ord a b = Order.Greater -> P (a::as) bs -> P (a::as) (b::bs))
-  (as bs: List α) : P as bs := 
-  List.sorted_intersect.induction.bounded
-    empty_left empty_right induct_lt induct_eq induct_gt
-    as bs (len as + len bs).inc (nat.lt_inc _)
-
-#print axioms List.sorted_intersect.induction
-
-theorem List.sorted_intersect.induction.unfuel
-  [Compare α] 
-  {P: List α -> List α -> Sort _}
-  (empty_left: ∀bs, P [] bs)
-  (empty_right: ∀as, P as [])
-  (induct_lt: ∀a as b bs, Compare.ord a b = Order.Less -> P as (b::bs) -> P (a::as) (b::bs))
-  (induct_eq: ∀a as b bs, Compare.ord a b = Order.Eq -> P as bs -> P (a::as) (b::bs))
-  (induct_gt: ∀a as b bs, Compare.ord a b = Order.Greater -> P (a::as) bs -> P (a::as) (b::bs))
-  (as bs: List α) : 
-  ∀fuel fuel_def,
-  List.sorted_intersect.induction.bounded 
-    empty_left empty_right induct_lt induct_eq induct_gt as bs fuel fuel_def =
-  List.sorted_intersect.induction 
-    empty_left empty_right induct_lt induct_eq induct_gt as bs := by
-  intro fuel fuel_def
-  unfold List.sorted_intersect.induction
-  rw [List.sorted_intersect.induction.bounded.fuel_irr]
-
-#print axioms List.sorted_intersect.induction.unfuel
+import Alg.ListProps.Sorted.Induction
 
 def List.sorted_intersect [Compare α] : List α -> List α -> List α := by
-  apply List.sorted_intersect.induction
+  apply List.sorted.induction
   {
     intro _
     exact []
@@ -208,7 +30,7 @@ def List.sorted_intersect [Compare α] : List α -> List α -> List α := by
 #print axioms List.sorted_intersect
 
 theorem List.sorted_intersect.empty_left [Compare α] : ∀{as bs: List α}, as = [] -> as.sorted_intersect bs = [] := by
-  apply List.sorted_intersect.induction
+  apply List.sorted.induction
 
   {
     intro bs _
@@ -231,7 +53,7 @@ theorem List.sorted_intersect.empty_left [Compare α] : ∀{as bs: List α}, as 
 #print axioms List.sorted_intersect.empty_left
 
 theorem List.sorted_intersect.empty_right [Compare α] : ∀{as bs: List α}, bs = [] -> as.sorted_intersect bs = [] := by
-  apply List.sorted_intersect.induction
+  apply List.sorted.induction
 
 
   {
@@ -255,7 +77,7 @@ theorem List.sorted_intersect.empty_right [Compare α] : ∀{as bs: List α}, bs
 #print axioms List.sorted_intersect.empty_right
 
 theorem List.sorted_intersect.induct_lt.helper [Compare α] : ∀(as bs cs ds: List α) (c d: α), as = c::cs -> bs = d::ds -> Compare.ord c d = Order.Less -> as.sorted_intersect bs = cs.sorted_intersect bs := by
-  apply List.sorted_intersect.induction
+  apply List.sorted.induction
 
   {
     intro bs
@@ -276,7 +98,7 @@ theorem List.sorted_intersect.induct_lt.helper [Compare α] : ∀(as bs cs ds: L
     have ⟨ b_eq_d, bs_eq_ds ⟩  := List.cons.inj bs_eq_ds
     conv => {
       lhs
-      unfold sorted_intersect induction induction.bounded
+      unfold sorted_intersect sorted.induction sorted.induction.bounded
     }
     simp
     rw [a_ord_b]
@@ -316,7 +138,7 @@ theorem List.sorted_intersect.induct_lt [Compare α] : ∀{a b: α} {as bs: List
 #print axioms List.sorted_intersect.induct_lt
 
 theorem List.sorted_intersect.induct_eq.helper [Compare α] : ∀(as bs cs ds: List α) (c d: α), as = c::cs -> bs = d::ds -> Compare.ord c d = Order.Eq -> as.sorted_intersect bs = c::(cs.sorted_intersect ds) := by
-  apply List.sorted_intersect.induction
+  apply List.sorted.induction
 
   {
     intro bs
@@ -347,7 +169,7 @@ theorem List.sorted_intersect.induct_eq.helper [Compare α] : ∀(as bs cs ds: L
     have ⟨ b_eq_d, bs_eq_ds ⟩  := List.cons.inj bs_eq_ds
     conv => {
       lhs
-      unfold sorted_intersect induction induction.bounded
+      unfold sorted_intersect sorted.induction sorted.induction.bounded
     }
     simp
     rw [a_ord_b]
@@ -355,8 +177,8 @@ theorem List.sorted_intersect.induct_eq.helper [Compare α] : ∀(as bs cs ds: L
     rw [a_eq_c, b_eq_d]
     rw [as_eq_cs, bs_eq_ds]
     simp
-    unfold sorted_intersect induction
-    rw [induction.bounded.fuel_irr]
+    unfold sorted_intersect sorted.induction
+    rw [sorted.induction.bounded.fuel_irr]
     rfl
   }
 
@@ -379,7 +201,7 @@ theorem List.sorted_intersect.induct_eq [Compare α] : ∀{a b: α} {as bs: List
 #print axioms List.sorted_intersect.induct_eq
 
 theorem List.sorted_intersect.induct_gt.helper [Compare α] : ∀(as bs cs ds: List α) (c d: α), as = c::cs -> bs = d::ds -> Compare.ord c d = Order.Greater -> as.sorted_intersect bs = as.sorted_intersect ds := by
-  apply List.sorted_intersect.induction
+  apply List.sorted.induction
 
   {
     intro bs
@@ -420,7 +242,7 @@ theorem List.sorted_intersect.induct_gt.helper [Compare α] : ∀(as bs cs ds: L
     have ⟨ b_eq_d, bs_eq_ds ⟩  := List.cons.inj bs_eq_ds
     conv => {
       lhs
-      unfold sorted_intersect induction induction.bounded
+      unfold sorted_intersect sorted.induction sorted.induction.bounded
     }
     simp
     rw [a_ord_b]
@@ -428,8 +250,8 @@ theorem List.sorted_intersect.induct_gt.helper [Compare α] : ∀(as bs cs ds: L
     rw [a_eq_c, b_eq_d]
     rw [as_eq_cs, bs_eq_ds]
     simp
-    unfold sorted_intersect induction
-    rw [induction.bounded.fuel_irr]
+    unfold sorted_intersect sorted.induction
+    rw [sorted.induction.bounded.fuel_irr]
     rfl
   }
 
@@ -447,7 +269,7 @@ theorem List.sorted_intersect.keeps_sorted.helper [Compare α] {x: α} :
   sorted (x::bs) ->
   sorted (sorted_intersect as bs) ->
   sorted (x :: sorted_intersect as bs) := by
-  apply induction
+  apply sorted.induction
   {
     intro _
     intro _ _ _
@@ -494,7 +316,7 @@ theorem List.sorted_intersect.keeps_sorted [Compare α] : ∀(as bs: List α),
   as.sorted ->
   bs.sorted ->
   (as.sorted_intersect bs).sorted := by
-  apply List.sorted_intersect.induction
+  apply List.sorted.induction
   {
     intro _
     intro _ _
@@ -544,7 +366,7 @@ theorem List.sorted_intersect.of_contains [Compare α] : ∀(as bs: List α) (x:
   as.sorted ->
   bs.sorted ->
   (as.sorted_intersect bs).containsP x := by
-  apply List.sorted_intersect.induction
+  apply List.sorted.induction
   {
     intro _
     intro _ _ _ _ _
@@ -625,7 +447,7 @@ theorem List.sorted_intersect.to_contains [Compare α] : ∀(as bs: List α) (x:
   (as.sorted_intersect bs).containsP x ->
   as.containsP x ∧ bs.containsP x 
    := by
-  apply List.sorted_intersect.induction
+  apply List.sorted.induction
   {
     intro _
     intro _ _ _ i_con
